Add TracesInform.v. So far, no shared memory is added to the call and return events because it is not needed for the back-translation function

Common/TracesInform.v
@@ -3,6 +3,8 @@ Require Import CompCert.Events.
 Require Import Common.Definitions.
 Require Import Common.Linking.
 Require Import Common.CompCertExtensions.
+Require Import Common.Values.
+Require Import Common.Traces.
 
 From mathcomp
   Require Import ssreflect ssrfun ssrbool eqtype ssrnat seq.
@@ -11,32 +13,52 @@ Set Implicit Arguments.
 Unset Strict Implicit.
 Unset Printing Implicit Defensive.
 
-(* The following section will need to be refactored out from both this file
-   and from Traces.v.
-*)
-Section Suffix.
+Inductive Eregister : Type :=
+  E_R_ONE | E_R_COM | E_R_AUX1 | E_R_AUX2 | E_R_RA | E_R_SP | E_R_ARG.
 
-Variable T : eqType.
+Inductive Ebinop : Set :=
+  Add : Ebinop | Minus : Ebinop | Mul : Ebinop | Eq : Ebinop | Leq : Ebinop.
 
-Implicit Types (x : T) (s : seq T).
+Inductive event_inform :=
+| ECall : Component.id -> Procedure.id -> value -> Component.id -> event_inform
+| ERet : Component.id -> value -> Component.id -> event_inform
+| EConst : Component.id -> value -> Eregister -> event_inform
+| EMov : Component.id -> Eregister -> Eregister -> event_inform
+| EBinop : Component.id -> Ebinop -> Eregister -> Eregister -> Eregister -> event_inform
+| ELoad : Component.id -> Eregister -> Eregister -> event_inform
+| EStore : Component.id -> Eregister -> Eregister -> event_inform
+| EAlloc : Component.id -> Eregister -> Eregister -> event_inform
+| EInvalidateRA : Component.id -> event_inform.
 
-Fixpoint suffix_rec s1 s2 : bool :=
-  (s1 == s2) ||
-  if s2 is x :: s2' then suffix_rec s1 s2' else false.
-
-Definition suffix := locked suffix_rec.
-
-Lemma suffix_refl : reflexive suffix.
-Proof. by case=> [|??]; rewrite /suffix -lock //= eqxx. Qed.
-
-Lemma suffix_cons s1 x s2 :
-  suffix s1 (x :: s2) = (s1 == x :: s2) || suffix s1 s2.
-Proof. by rewrite /suffix; unlock. Qed.
-
-Lemma suffix_nil s1 : suffix s1 [::] = (s1 == [::]).
-Proof. by rewrite /suffix -lock /= orbF. Qed.
-
-End Suffix.
+Instance event_inform_EventClass : EventClass event_inform :=
+  {
+    cur_comp_of_event e :=
+      match e with
+      | ECall   C _ _ _ => C
+      | ERet    C _ _   => C
+      | EConst  C _ _ => C
+      | EMov    C _ _ => C
+      | EBinop  C _ _ _ _ => C
+      | ELoad   C _ _ => C
+      | EStore  C _ _ => C
+      | EAlloc  C _ _ => C
+      | EInvalidateRA C => C
+      end;
+    next_comp_of_event e :=
+      match e with
+      (* Calls and returns yield control. *)
+      | ECall  _ _ _ C => C
+      | ERet   _ _   C => C
+      (* All the other events retain control. *)
+      | EConst  C _ _ => C
+      | EMov    C _ _ => C
+      | EBinop  C _ _ _ _ => C
+      | ELoad   C _ _ => C
+      | EStore  C _ _ => C
+      | EAlloc  C _ _ => C
+      | EInvalidateRA C => C
+      end
+  }.
 
 Section Traces.
 
@@ -50,7 +72,8 @@ Inductive stack_state := StackState {
 
 Definition stack_state0 := StackState Component.main [::].
 
-Implicit Types (t : trace) (C : Component.id) (s : stack_state) (intf : Program.interface).
+Implicit Types (t : trace event_inform)
+         (C : Component.id) (s : stack_state) (intf : Program.interface).
 
 Fixpoint well_bracketed_trace s t : bool :=
   match t with
@@ -86,13 +109,13 @@ Lemma well_bracketed_trace_cat s t1 t2 :
   well_bracketed_trace s (t1 ++ t2) =
   well_bracketed_trace s t1 &&
   well_bracketed_trace (run_trace s t1) t2.
-Proof.  
-(* TODO: Try to understand and fix the proof. *)
-elim: t1 s=> [//|[C ? ? C'|C ? C'|? ? ?|? ? ?] t1 IH] [Ccur callers] /=.
-  by rewrite IH andbA.
-case: eqP callers => [_ {Ccur}|_] //= [|top callers] //=.
-  by rewrite IH andbA.
-Admitted.
+Proof.
+  elim: t1 s=> [//|[C ? ? C'|C ? C'|? ? ?|? ? ?|? ? ? ? ?|? ? ?|? ? ?|? ? ?|?] t1 IH]
+                 [Ccur callers] /=;
+  try by rewrite IH andbA.
+case: eqP callers => [_ {Ccur}|_] //= [|top callers] //=;
+  by rewrite IH andbA.                
+Qed.
 
 Definition seq_of_stack_state s := cur_comp s :: callers s.
 
@@ -106,31 +129,40 @@ Lemma well_bracketed_trace_suffix t C C' Cs :
   suffix [:: C, C' & Cs] (run_trace stack_state0 t) ->
   exists t1 P arg t2, t = t1 ++ ECall C' P arg C :: t2.
 Proof.
-(* TODO: Try to understand and fix the proof. *)
-set s0 := stack_state0.
-elim/last_ind: t=> [|t e IH] //=.
-  by rewrite suffix_cons suffix_nil /= orbF => _ /eqP.
-have -> : well_bracketed_trace s0 (rcons t e) =
-          well_bracketed_trace s0 t &&
-          well_bracketed_trace (run_trace s0 t) [:: e].
-  by rewrite -cats1 well_bracketed_trace_cat andbC.
-rewrite run_trace1; case: e => [C1 P arg C2|C1 ? C2|? ? ?|? ? ?] /=.
-  rewrite andbT; case/andP=> wb_t /eqP <- {C1} /=.
-  rewrite -[_ :: callers _]/(run_trace s0 t : seq _) suffix_cons /=.
-  case/orP=> [/eqP|Hsuff].
-    case: (run_trace _ _)=> [? ?] [<- <- <-] /=.
-    by eexists t, _, _, [::]; rewrite cats1.
-  case/(_ wb_t Hsuff): IH=> [t1 [P' [arg' [t2 ->]]]].
-  by eexists t1, P', arg', (rcons t2 _); rewrite rcons_cat; split; eauto.
-case/and3P=> wb_t /eqP e1 e2.
-have -> : StackState C2 (tl (callers (run_trace s0 t))) =
-          callers (run_trace s0 t) :> seq _.
-  by case: (callers _) e2=> [|e cs] //= /andP [/eqP ->].
-move=> Hsuff; have {Hsuff} Hsuff: suffix [:: C, C' & Cs] (run_trace s0 t).
-  by rewrite suffix_cons Hsuff orbT.
-case/(_ wb_t Hsuff): IH=> [t1 [P [arg [t2 ->]]]].
-  by eexists t1, P, arg, (rcons _ _); rewrite rcons_cat.
-Admitted.
+  set s0 := stack_state0.
+  elim/last_ind: t=> [|t e IH] //=.
+    by rewrite suffix_cons suffix_nil /= orbF => _ /eqP.
+    have -> : well_bracketed_trace s0 (rcons t e) =
+              well_bracketed_trace s0 t &&
+                                   well_bracketed_trace (run_trace s0 t) [:: e].
+      by rewrite -cats1 well_bracketed_trace_cat andbC.
+      rewrite run_trace1;
+        case: e => [C1 P arg C2|C1 ? C2|C1 ? ?|C1 ? ?|C1 ? ? ? ?|C1 ? ?|C1 ? ?|C1 ? ?|C1]
+                     /=;
+                     try rewrite andbT;
+                     try (case/andP=> wb_t /eqP <- {C1} /=;
+                                           move => Hsuff;
+                                                   case/(_ wb_t Hsuff):
+                                                     IH=> [t1 [P' [arg' [t2 ->]]]];
+                                                            by eexists
+                                                                 t1, P', arg', (rcons t2 _);
+                                                            rewrite rcons_cat; split; eauto).
+  - case/andP=> wb_t /eqP <- {C1} /=.
+    rewrite -[_ :: callers _]/(run_trace s0 t : seq _) suffix_cons /=.
+    case/orP=> [/eqP|Hsuff].
+    + case: (run_trace _ _)=> [? ?] [<- <- <-] /=.
+        by eexists t, _, _, [::]; rewrite cats1.
+    + case/(_ wb_t Hsuff): IH=> [t1 [P' [arg' [t2 ->]]]].
+        by eexists t1, P', arg', (rcons t2 _); rewrite rcons_cat; split; eauto.
+  - case/and3P=> wb_t /eqP e1 e2.
+    have -> : StackState C2 (tl (callers (run_trace s0 t))) =
+              callers (run_trace s0 t) :> seq _.
+      by case: (callers _) e2=> [|e cs] //= /andP [/eqP ->].
+      move=> Hsuff; have {Hsuff} Hsuff: suffix [:: C, C' & Cs] (run_trace s0 t).
+        by rewrite suffix_cons Hsuff orbT.
+        case/(_ wb_t Hsuff): IH=> [t1 [P [arg [t2 ->]]]].
+          by eexists t1, P, arg, (rcons _ _); rewrite rcons_cat.
+Qed.
 
 Lemma well_bracketed_trace_inv t C res C' :
   well_bracketed_trace stack_state0 (t ++ [:: ERet C res C']) ->
@@ -154,15 +186,14 @@ Qed.
    Only then can we use reachability to compute the views of each component.
    Based on the view of a component memory, we can judge whether an ERead/EWrite that it
    performs is a possible read/write.  *)
-Definition well_formed_event intf (e: event) : bool :=
+Definition well_formed_event intf (e: event_inform) : bool :=
   match e with
   | ECall C P _ C' => (C != C') && imported_procedure_b intf C C' P
   | ERet  C _   C' => (C != C')
-  | ERead _ _ _ => false
-  | EWrite _ _ _ => false
+  | _ => true
   end.
 
-Definition well_formed_trace intf (t: trace) : bool :=
+Definition well_formed_trace intf (t: trace event_inform) : bool :=
   well_bracketed_trace stack_state0 t &&
   all (well_formed_event intf) t.
 
@@ -177,19 +208,23 @@ Lemma well_formed_trace_int intf t :
 Proof.
 Admitted.
 (*
-case/andP=> wb wf clos; rewrite /declared_event_comps.
-apply/allP; case=> [C P v C'|C v C'] /=; rewrite !mem_domm.
-- move/(allP wf)=> /andP [_ imp].
-  move: (imp); rewrite /imported_procedure_b; case: getm => //= _ _.
-  by case/imported_procedure_iff/clos: imp=> ? [->].
-- move=> in_p; case/path.splitP: in_p wb wf => {t} t1 t2.
-  rewrite -cats1 /= well_bracketed_trace_cat.
-  case/andP=> /well_bracketed_trace_inv [t11 [P [v' [t12 ->]]]] _ wf.
-  have : well_formed_event intf (ECall C' P v' C).
-    by move/allP: wf; apply; rewrite !mem_cat inE eqxx /= orbT.
-  case/andP=> _ imp.
-  case/imported_procedure_iff/clos: (imp)=> ? [-> _] /=.
-  by move: imp; rewrite /imported_procedure_b; case: getm.
+  case/andP=> wb wf clos; rewrite /declared_event_comps.
+  Check allP.
+  Check pred_sort.
+  assert (forall x, x \in t -> (cur_comp_of_event x \in domm intf)
+                                 && (next_comp_of_event x \in domm intf) x) as asrt.
+  case=> [C P v C'|C v C'] /=; rewrite !mem_domm.
+  - move/(allP wf)=> /andP [_ imp].
+    move: (imp); rewrite /imported_procedure_b; case: getm => //= _ _.
+      by case/imported_procedure_iff/clos: imp=> ? [->].
+  - move=> in_p; case/path.splitP: in_p wb wf => {t} t1 t2.
+    rewrite -cats1 /= well_bracketed_trace_cat.
+    case/andP=> /well_bracketed_trace_inv [t11 [P [v' [t12 ->]]]] _ wf.
+    have : well_formed_event intf (ECall C' P v' C).
+      by move/allP: wf; apply; rewrite !mem_cat inE eqxx /= orbT.
+      case/andP=> _ imp.
+      case/imported_procedure_iff/clos: (imp)=> ? [-> _] /=.
+        by move: imp; rewrite /imported_procedure_b; case: getm.
 Qed.
 *)
 End Traces.
